Prove the correctness of captures utility.

RegexCorrectness/Regex/Captures.lean
@@ -3,17 +3,22 @@ import RegexCorrectness.Regex.Basic
 
 set_option autoImplicit false
 
+open String (Pos)
+
+def Regex.CapturedGroups.Spec {re : Regex} (s : re.IsSearchRegex) (self : CapturedGroups) : Prop :=
+  ∃ l m r groups,
+    s.expr.Captures ⟨l, [], m ++ r⟩ ⟨l, m.reverse, r⟩ groups ∧
+    self.get 0 = .some (⟨String.utf8Len l⟩, ⟨String.utf8Len l + String.utf8Len m⟩) ∧
+    ∀ i, self.get i = NFA.materializeRegexGroups groups i
+
 namespace Regex.Captures
 
 def Valid (self : Captures) : Prop :=
   self.regex.IsSearchRegex ∧ self.currentPos.Valid self.haystack
 
-theorem next?_some {self self' : Captures} {captured} (h : self.next? = .some (captured, self'))
+theorem captures_of_next?_some {self self' : Captures} {captured} (h : self.next? = .some (captured, self'))
   (v : self.Valid) :
-  self'.Valid ∧
-  ∃ l m r groups,
-    v.1.expr.Captures ⟨l, [], m ++ r⟩ ⟨l, m.reverse, r⟩ groups ∧
-    ∀ i, captured.get i = NFA.materializeRegexGroups groups i := by
+  self'.Valid ∧ captured.Spec v.1 := by
   unfold next? at h
   split at h
   next lt =>
@@ -22,7 +27,8 @@ theorem next?_some {self self' : Captures} {captured} (h : self.next? = .some (c
     | none => simp at h
     | some matched =>
       have : 1 ≤ self.regex.maxTag := v.1.le_maxTag
-      have ⟨l, m, r, groups, c, eqv, eq₁, eq₂⟩ := v.1.captures_of_captureNext h' v.2 (by omega)
+      have ⟨l, m, r, groups, eqstring, c, eqv, eq₁, eq₂⟩ :=
+        v.1.captures_of_captureNext h' v.2 (by omega)
 
       simp at h
       set captured' := CapturedGroups.mk matched.val
@@ -70,7 +76,7 @@ theorem next?_some {self self' : Captures} {captured} (h : self.next? = .some (c
             have := v.1.maxTag_eq ▸ NFA.lt_of_mem_tags_compile v.1.nfa_eq.symm this
             simp at h₁
             omega
-      have : captured'.get 0 = .some (⟨String.utf8Len l⟩, ⟨String.utf8Len l + String.utf8Len m⟩) := by
+      have captured₀ : captured'.get 0 = .some (⟨String.utf8Len l⟩, ⟨String.utf8Len l + String.utf8Len m⟩) := by
         simp [hcaptured 0]
         have h₁ := (eqv 0).1 (by omega)
         have h₂ := (eqv 0).2 (by omega)
@@ -80,17 +86,48 @@ theorem next?_some {self self' : Captures} {captured} (h : self.next? = .some (c
         have ⟨_, eq₂⟩ := h₂
         simp [eq₂] at eq₁
         simp [eq₁, eq₂]
-      simp [this] at h
+      simp [captured₀] at h
       split at h
       next =>
         simp at h
         simp [←h, Valid]
-        -- TODO: requires `self.haystack = l ++ m ++ r` so that the position `⟨l ++ m⟩` is valid
-        exact ⟨⟨v.1, sorry⟩, l, m, r, groups, c, hcaptured⟩
+        have vp : Pos.Valid self.haystack ⟨String.utf8Len l + String.utf8Len m⟩ := by
+          refine ⟨l ++ m, r, ?_, by simp⟩
+          simp at eqstring
+          simp [eqstring]
+        exact ⟨⟨v.1, vp⟩, l, m, r, groups, c, captured₀, hcaptured⟩
       next nlt =>
         simp at h
         simp [←h, Valid]
-        exact ⟨⟨v.1, String.valid_next v.2 lt⟩, l, m, r, groups, c, hcaptured⟩
+        exact ⟨⟨v.1, String.valid_next v.2 lt⟩, l, m, r, groups, c, captured₀, hcaptured⟩
   next => simp at h
+
+theorem regex_eq_of_next?_some {self self' : Captures} {captured} (h : self.next? = .some (captured, self')) :
+  self'.regex = self.regex := by
+  unfold next? at h
+  split at h
+  next =>
+    simp at h
+    set captured' := VM.captureNext self.regex.nfa self.regex.wf (self.regex.maxTag + 1) ⟨self.haystack, self.currentPos⟩
+    match h' : captured' with
+    | none => simp at h
+    | some buffer =>
+      simp at h
+      match h'' : CapturedGroups.get ⟨buffer.val⟩ 0 with
+      | none => simp [h''] at h
+      | some _ =>
+        simp [h''] at h
+        split at h
+        next =>
+          simp at h
+          simp [←h]
+        next =>
+          simp at h
+          simp [←h]
+  next => simp at h
+
+theorem valid_captures {re : Regex} (haystack : String) (s : re.IsSearchRegex) :
+  (re.captures haystack).Valid :=
+  ⟨s, haystack.valid_mkIterator⟩
 
 end Regex.Captures
