RegexCorrectness/VM/Correspondence/Correctness.lean
@@ -14,12 +14,13 @@ theorem captureNext_correct {e nfa wf bufferSize it matched}
   (eq : NFA.compile e = nfa) (disj : e.Disjoint)
   (h : captureNext nfa wf bufferSize it = matched) (v : it.Valid) (isSome : matched.isSome) :
   ∃ l m r groups,
+    it.toString = ⟨l ++ m ++ r⟩ ∧
     e.Captures ⟨l, [], m ++ r⟩ ⟨l, m.reverse, r⟩ groups ∧
     EquivMaterializedUpdate (materializeRegexGroups groups) (matched.get isSome) := by
   generalize h' : captureNext' nfa wf it = matched'
   have refMatched : refineUpdateOpt matched' matched := h' ▸ h ▸ captureNext'.refines
   have isSome' := (refineUpdateOpt.isSome_iff refMatched).mpr isSome
-  have ⟨l, r, span, groups, eqv, c⟩ := captures_of_captureNext'_some eq h' v isSome'
+  have ⟨l, r, span, groups, eqstring, c, eqv⟩ := captures_of_captureNext'_some eq h' v isSome'
   have ⟨m, eql, eqm, eqr⟩ := c.span_eq
   simp at eql eqm eqr
   subst r
@@ -27,11 +28,13 @@ theorem captureNext_correct {e nfa wf bufferSize it matched}
     calc
       _ = (⟨span.l, span.m, span.r⟩ : Span) := rfl
       _ = ⟨l, m.reverse, span.r⟩ := by simp [eql, eqm]
+  rw [eqspan, Span.toString] at eqstring
+  simp at eqstring
   have eqv' : EquivMaterializedUpdate (materializeRegexGroups groups) (materializeUpdates bufferSize (matched'.get isSome')) :=
     eqv.materialize c disj
   have eq : matched = .some (matched.get isSome) := by simp
   have eq' : matched' = .some (matched'.get isSome') := by simp
   rw [eq, eq', refineUpdateOpt] at refMatched
-  exact ⟨l, m, span.r, groups, eqspan ▸ c, refMatched ▸ eqv'⟩
+  exact ⟨l, m, span.r, groups, by simp [←eqstring], eqspan ▸ c, refMatched ▸ eqv'⟩
 
 end Regex.VM
